Added timing

Print.thy
@@ -2,22 +2,68 @@ theory Print
   imports Show.Show_Instances "HOL-Library.Code_Char"
 begin
 
+subsection \<open>Printing\<close>
+
 text \<open>Taken from AFP-entry "Affine-Arithmetic".\<close>
 
 definition print_raw :: "String.literal \<Rightarrow> unit" where "print_raw x = ()"
+
+abbreviation "print \<equiv> (\<lambda>a b. let _ = print_raw (String.implode (show a)) in b)"
+
+definition echo :: "'a \<Rightarrow> 'a::show" where "echo x = print x x"
+
+code_printing constant print_raw \<rightharpoonup> (SML) "writeln"
+
+lemma echo_id: "echo = (\<lambda>x. x)"
+  by (rule, simp add: echo_def)
+
+subsection \<open>File Output\<close>
 
 definition file_output :: "String.literal \<Rightarrow> ((String.literal \<Rightarrow> unit) \<Rightarrow> 'a) \<Rightarrow> 'a" where
   "file_output _ f = f (\<lambda>_. ())"
 
 code_printing constant file_output \<rightharpoonup> (SML) "(fn s => fn f => File.open'_output (fn os => f (File.output os)) (Path.explode s))"
 
-abbreviation "print \<equiv> print_raw \<circ> String.implode \<circ> show"
+subsection \<open>Timing\<close>
 
-definition echo :: "'a \<Rightarrow> 'a::show" where "echo x = (let _ = print x in x)"
+typedecl ('a, 'b) cpu_timer
+typedecl time
 
-code_printing constant print_raw \<rightharpoonup> (SML) "writeln"
+consts start_cpu_timer :: "unit \<Rightarrow> ('a, 'b) cpu_timer"
+consts check_cpu_timer :: "('a, 'b) cpu_timer \<Rightarrow> (time \<times> time)"
+consts time_to_string :: "time \<Rightarrow> String.literal"
 
-lemma echo_id: "echo = (\<lambda>x. x)"
-  by (rule, simp add: echo_def)
+definition check_cpu_timer_string :: "('a, 'b) cpu_timer \<Rightarrow> String.literal"
+  where "check_cpu_timer_string t =
+    (let (usr, sys) = check_cpu_timer t in (STR (''User: '') + time_to_string usr) + STR (''  System: '') + time_to_string sys)"
+
+definition timing_raw :: "String.literal \<Rightarrow> (unit \<Rightarrow> 'a) \<Rightarrow> 'a"
+  where "timing_raw s f = (let tmr = (start_cpu_timer ())::(nat, nat) cpu_timer;
+                         res = f ();
+                         _ = print_raw (s + check_cpu_timer_string tmr) in res)"
+
+definition timing_raw_nores :: "String.literal \<Rightarrow> (unit \<Rightarrow> 'a) \<Rightarrow> unit"
+  where "timing_raw_nores s f = (let tmr = (start_cpu_timer ())::(nat, nat) cpu_timer;
+                         res = f ();
+                         _ = print_raw (s + check_cpu_timer_string tmr) in ())"
+
+abbreviation "timing \<equiv> (\<lambda>v. timing_raw (STR '''') (\<lambda>_. v))"
+abbreviation "timing_nores \<equiv> (\<lambda>v. timing_raw_nores (STR '''') (\<lambda>_. v))"
+abbreviation "timing_lbl \<equiv> (\<lambda>s v. timing_raw (String.implode s + STR '': '') (\<lambda>_. v))"
+
+lemma timing_raw_id: "timing_raw s f = f ()"
+  by (simp add: timing_raw_def)
+
+code_printing
+type_constructor cpu_timer \<rightharpoonup>
+    (SML) "_ Timer.cpu_timer"
+| type_constructor time \<rightharpoonup>
+    (SML) "Time.time"
+| constant start_cpu_timer \<rightharpoonup>
+    (SML) "Timer.startCPUTimer"
+| constant check_cpu_timer \<rightharpoonup>
+    (SML) "(fn ct => (let val {usr, sys} = Timer.checkCPUTimer ct in (usr, sys) end))"
+| constant time_to_string \<rightharpoonup>
+    (SML) "Time.toString"
 
 end (* theory *)
